Fix metavariable bug

tests/lean/run/cbv1.lean
@@ -4,7 +4,7 @@ inductive myNat where
   | myZero : myNat
   | mySucc : myNat → myNat
 
-def myId (n : Nat) : Nat := n
+def myId (n : myNat) : myNat := n
 
 def natFun (n : myNat) : myNat := match n with
   | .myZero => .myZero
@@ -15,14 +15,21 @@ def myRev (b : Bool) : Nat := match b with
   | true => .zero
   | false => Nat.zero.succ
 
-theorem myTest0 : natFun (myNat.myZero.mySucc.mySucc) = myNat.myZero := by
+theorem myTest0 : natFun (myNat.myZero.mySucc.mySucc.mySucc.mySucc) = (myNat.myZero.mySucc.mySucc.mySucc.mySucc) := by
   conv =>
     lhs
     cbv
     cbv
+    cbv
+    cbv
+    cbv
+
+
+theorem myTest1 : (myId .myZero).mySucc.mySucc = myNat.myZero := by
+  conv =>
+    lhs
+    cbv
   sorry
-
-
 
 
 
